\documentclass[a4paper,11pt]{article}
\usepackage[a4paper, margin=20mm]{geometry}
\usepackage[T1]{fontenc}
\usepackage[utf8]{inputenc}
\usepackage{mathfunc}

% Header
% ===========================

\title{Conditional Probability}
\author{Sheldon Ross, A First Course in Probability (Chapter 3)}
\date{May 29\textsuperscript{th}, 2015}


% Document
% ===========================

\begin{document}
\maketitle
\pagenumbering{gobble}

\begin{outline}

  \dbullet{3.2.1}
    If \(\bbp(F) > 0\), then \(\bbp(E|F) = \frac{\bbp(EF)}{\bbp(F)}\).
    
  \tbullet{3.2.2}
    \(\bbp(\inflatedot[]{E}{n}) = \bbp(E_1)\bbp(E_2|E_1)\ldots\bbp(E_n|\inflatedot[]{E}{n-1})\).
    
  \tbullet{3.3.1}
    \(\bbp(E) = \bbp(E|F)\bbp(F) + \bbp(E|F^c)\bbp(F^c)\)
    
    \begin{proof}
      Note the following:
      \begin{align*}
        \bbp(E) &= \bbp(EF \cup EF^c)    \\
                &= \bbp(EF) + \bbp(EF^c) \\
                &= \bbp(E|F)\bbp(F)      \\
                &= \bbp(E|F^c)\bbp(F^c)
      \end{align*}
    \end{proof}
    
  \tbullet{3.3.2}
    The "odds" of an event \(A\) are defined by \(\frac{\bbp(A)}{\bbp(A^c)}\). That is,
    how much more likely it is event \(A\) occurs than it is that it doesn't.

  \pbullet{3.3.3}
    The new odds after evidence \(E\) is introduced are
    \[
      \frac{\bbp(H|E)}{\bbp(H^c|E)} = 
      \frac{\bbp(H)\bbp(E|H)}{\bbp(H^c)\bbp(E|H^c)}
      \text{.}
    \]
    
    \begin{proof}
      Note the following:
      \begin{align*}
        \bbp(H|E)   &= \frac{\bbp(E|H)\bbp(H)}{\bbp(E)}\\
        \bbp(H^c|E) &= \frac{\bbp(E|H^c)\bbp(H^c)}{\bbp(E)}
      \end{align*}
      Divide two equations above for answer.
    \end{proof}

  \pbullet{3.3.4}
    Suppose \(\inflatedot{F}{n}\) are mutually exclusive events such that \(\bigcup_{i=1}^n F_i = S\). Then
    \(\bbp(E) = \sum_{i=1}^n \bbp(E|F_i)\bbp(F_i)\).
    
  \tbullet{3.3.5 (Bayes's Theorem)}
    Let \(\inflatedot{F}{n}\) be mutually exclusive, exhaustive events. Then given event \(E\),
    \begin{align*}
      \bbp(F_j|E) &= \frac{\bbp(EF_j)}{\bbp(E)} \\
                        &= \frac{\bbp(E|F_j)\bbp(F_j)}{\sum_{i=1}^n \bbp(E|F_i)\bbp(F_i)}
                           \text{.}
    \end{align*}

  \dbullet{3.4.1}
    Two events \(E\) and \(F\) are said to be "independent" if \(\bbp(EF) = \bbp(E)\bbp(F)\).
    Two events that are not independent are said to be dependent.
    
  \pbullet{3.4.2}
    If \(E\) and \(F\) are independent, then so are \(E\) and \(F^c\).
    
    \begin{proof}
      Assume \(E\) and \(F\) are independent. Since
      \begin{align*}
                    E &= EF \cup EF^c \Rightarrow   \\
        \bbp(E) &=\bbp(EF) + \bbp(EF^c)             \\
                      &= \bbp(E)\bbp(F) + \bbp(EF^c)
      \end{align*}
      Thus
      \begin{align*}
        \bbp(EF^c) &= \bbp(E) - \bbp(E)\bbp(F)\\
                         &= \bbp(E)[1-\bbp(F)]\\
                         &= \bbp(E)\bbp(F^c)
      \end{align*}
    \end{proof}

  \dbullet{3.4.3}
    Three events \(E, F,\) and \(G\) are said to be independent if 
    \begin{align*}
      \bbp(EFG) &= \bbp(E)\bbp(F)\bbp(G),       \\
      \bbp(EF)  &= \bbp(E)\bbp(F),              \\
      \bbp(EG)  &= \bbp(E)\bbp(G), \text{ and } \\
      \bbp(FG)  &= \bbp(F)\bbp(G)
    \end{align*}
    
  \dbullet{3.4.4}
    The events \(\inflatedot{E}{n}\) are said to be independent if for every subset \(E_{1'}, E_{2'}, \ldots,
    E_{r'}\), \(r \leq n\), of these events, \(\bbp(E_{1'}E_{2'}\ldots E_{r'}) = \bbp(E_{1'})\bbp(E_{2'})
    \ldots\bbp(E_{r'})\). An infinite set of events are independent if every finite subset of those events
    is independent.
    
  \pbullet{3.5.1}
    Conditional probabilities satisfy the axioms of probability:
    \begin{enumerate}[i.]
      \item \(0 \leq \bbp(E|F) \leq 1\)
      \item \(\bbp(S|F) = 1\)
      \item If \(E_i, i = 1, \ldots\), are mutually exclusive events, then \(\bbp(\bigcup_{1}^{\infty}E_i|F) =
      \sum_{1}^{\infty}\bbp(E_i|F)\).
    \end{enumerate}

    \begin{proof}
      \begin{enumerate}[i.]
        \item
          Note \(0 \leq \bbp(E|F)\) is obvious. Now \(\bbp(E|F) = \frac{\bbp(EF)}{\bbp(F)}\) and note
          \(EF \subset F\). Thus \(\bbp(EF) \leq \bbp(F)\).
        \item
          \(\bbp(S|F) = \frac{\bbp(SF)}{\bbp(F)} = \frac{\bbp(F)}{\bbp(F)} = 1\).
        \item
          \(\bbp(\bigcup_{1}^{\infty} E_i|F) = \frac{\bbp([\bigcup_{1}^{\infty} E_i]F)}{\bbp(F)}
          = \frac{\bbp(\bigcup_{1}^{\infty}E_iF)}{\bbp(F)}\). This in turn is
          \(\frac{\sum_{1}^{\infty} \bbp(E_iF)}{\bbp(F)} = \sum\limits_{1}^{\infty} \frac{\bbp(E_iF)}{\bbp(F)}\).
      \end{enumerate}
    \end{proof}
\end{outline}

\end{document}
