\documentclass[a4paper,8pt]{article}
\usepackage[a4paper, margin=15mm]{geometry}
\usepackage[T1]{fontenc}
\usepackage[utf8]{inputenc}
\usepackage{mathfunc}

% Header
% ===========================

\title{Appendix: Logical Equivalences}
\author{Discrete Math and Its Applications by Kenneth H. Rosen (Chapter 1)}
\date{June 18\textsuperscript{th}, 2015}


% Document
% ===========================

\begin{document}
\maketitle
\pagenumbering{gobble}

\begin{outline}

  \tbullet{1.3.1 (Logical Equivalences)}
    \begin{enumerate}
      \begin{minipage}[t]{.5\textwidth}
        \item \textit{Identity Laws:}
          \begin{enumerate}[i.]
            \item \(p \wedge T \equiv p\)
            \item \(p \vee F \equiv p\)
          \end{enumerate}
        \item \textit{Domination Laws:}
          \begin{enumerate}[i.]
            \item \(p \vee T \equiv T\)
            \item \(p \wedge F \equiv F\)
          \end{enumerate}
        \item \textit{Idempotent Laws:}
          \begin{enumerate}[i.]
            \item \(p \vee p \equiv p\)
            \item \(p \wedge p \equiv p\)
          \end{enumerate}
        \item \textit{Commutative Laws:}
          \begin{enumerate}[i.]
            \item \(p \vee p \equiv q \vee p\)
            \item \(p \wedge p \equiv q \wedge p\)
          \end{enumerate}
        \item \textit{Associative Laws:}
          \begin{enumerate}[i.]
            \item \((p \vee q) \vee r \equiv p \vee (q \vee r)\)
            \item \((p \wedge q) \wedge r \equiv p \wedge (q \wedge r)\)
          \end{enumerate}
      \end{minipage}%
      \begin{minipage}[t]{.5\textwidth}
        \item \textit{Distributive Laws:}
          \begin{enumerate}[i.]
            \item \(p \vee (q \wedge r) \equiv (p \vee q) \wedge (p \vee r)\)
            \item \(p \wedge (q \vee r) \equiv (p \wedge q) \vee (p \wedge r)\)
          \end{enumerate}
        \item \textit{De Morgan's Laws:}
          \begin{enumerate}[i.]
            \item \(\neg(p \wedge q) \equiv \neg p \vee \neg q\)
            \item \(\neg(p \vee q) \equiv \neg p \wedge \neg q\)
          \end{enumerate}
        \item \textit{Absorption Laws:}
          \begin{enumerate}[i.]
            \item \(p \vee (p \wedge q) \equiv p\)
            \item \(p \wedge (p \vee q) \equiv p\)
          \end{enumerate}
        \item \textit{Negation Laws:}
          \begin{enumerate}[i.]
            \item \(p \vee \neg{p} \equiv T\)
            \item \(p \wedge \neg{p} \equiv F\)
          \end{enumerate}
      \end{minipage}
    \end{enumerate}

  \tbullet{1.3.2 (Logical Conditional Equivalences)}
    \begin{enumerate}
      \item \(p \rightarrow q \equiv \neg{p} \vee q\)
      \item \(p \rightarrow q \equiv \neg{q} \rightarrow \neg{p}\)
      \item \(p \vee q \equiv \neg p \rightarrow q\)
      \item \(p \wedge q \equiv \neg(p \rightarrow \neg q)\)
      \item \(\neg(p \rightarrow q) \equiv p \wedge \neg q\)
      \item \((p \rightarrow q) \wedge (p \rightarrow r) \equiv p \rightarrow (q \wedge r)\)
      \item \((p \rightarrow r) \wedge (q \rightarrow r) \equiv (p \vee q) \rightarrow r\)
      \item \((p \rightarrow q) \vee (p \rightarrow r) \equiv p \rightarrow (q \vee r)\)
      \item \((p \rightarrow r) \vee (q \rightarrow r) \equiv (p \wedge q) \rightarrow r\)
    \end{enumerate}

  \tbullet{1.3.3 (Logical Biconditional Statements)}
    \begin{enumerate}
      \item \(p \leftrightarrow q \equiv (p \rightarrow q) \wedge (q \rightarrow p)\)
      \item \(p \leftrightarrow q \equiv \neg p \leftrightarrow \neg q\)
      \item \(p \leftrightarrow q \equiv (p \wedge q) \vee (\neg p \wedge \neg q)\)
      \item \(\neg(p \leftrightarrow q) \equiv p \leftrightarrow \neg q\)
    \end{enumerate}

\end{outline}

\end{document}
