\documentclass[a4paper,11pt]{article}
\usepackage[a4paper, margin=20mm]{geometry}
\usepackage[T1]{fontenc}
\usepackage[utf8]{inputenc}
\usepackage{mathfunc}

% Header
% ===========================

\title{Parametric Equations and Polar Coordinates}
\author{Calculus Early Transcendentals by James Stewart (Chapter 10)}
\date{June 14\textsuperscript{th}, 2015}


% Document
% ===========================

\begin{document}
\maketitle
\pagenumbering{gobble}

\begin{outline}

  \tbullet{10.2.1 (Parametric to Cartesian)}
    If \(f'\) is continuous and \(f'(t) \neq 0\) for \(a \leq t \leq b\), then the parametric curve \(x = f(t),
    y = g(t), a \leq t \leq b\), can be put in the form \(y = F(x)\).
    
    \begin{proof}
      We note that if \(f'\) is continuous and \(f'(t) \neq 0\), then by the contrapositive of Fermat's Theorem, 
      there are no local minimums or maximums. In other words, \(f\) must be monotonically increasing or decreasing
      and as such, must be invertible. Thus \[f^{-1}(x) = t \Rightarrow y = g(t) = g(f^{-1}(x)) = F(x)\text{.}\]
    \end{proof}
    
  \tbullet{10.2.2 (Derivative of Parametric Curve)}
    Let \(x = f(t)\) and \(y = g(t)\) such that the conditions in Theorem 10.2.1 are satisfied (in a piecewise
    manner if necessary). Then \(y\) can be written as \(y = F(x)\), for some function \(F\) obtained by eliminating 
    the \(t\) parameter and \[ F'(x) = \frac{g'(t)}{f'(t)}\text{.} \]
    
    \begin{proof}
      Note \(y = F(x)\) can be written as \[ g(t) = F(f(t)) \] and so, if \(f, F,\) and \(f\) are differentiable, 
      the Chain Rules gives \[ g'(t) = F'(f(t))f'(t) = F'(x)f(t)\text{.} \] Thus, if \(f'(t) \neq 0\), we can 
      solve for \(F'(x)\): \[ F'(x) = \frac{g'(t)}{f'(t)}\text{.} \]
    \end{proof}

\end{outline}

\end{document}
